More refactorings/cleanups

common/theories/LoopChecking/OldPresentation.v
@@ -11,6 +11,33 @@
        C := relations_of_clauses cls |}.
 
 
+  Definition entails_cstr cstrs c :=
+    entails_clauses (to_clauses cstrs) (LoopCheck.to_clauses (to_constraint c)).
+
+  Definition entails_z_cstr cstrs c :=
+    entails_clauses (of_z_constraints cstrs) (LoopCheck.to_clauses c).
+
+  Definition entails_cstrs cstrs cstrs' :=
+    entails_clauses (of_z_constraints cstrs) (of_z_constraints cstrs').
+
+
+  Lemma check_valid m c :
+    check m c <-> entails_cstr (constraints m) c.
+  Proof.
+    rewrite /check LoopCheck.check_spec.
+    rewrite /entails_clauses.
+    enough ((LoopCheck.clauses (model m)) =_clset (to_clauses (constraints m))).
+    { split; intros ? ?.
+      move/H0. now rewrite H.
+      move/H0. now rewrite H. }
+    intros cl.
+    rewrite to_clauses_spec.
+    split.
+    - now move/(repr_constraints_inv m).
+    - intros [cstr [hin incl]].
+      eapply (repr_constraints m); tea.
+  Qed.
+
   Lemma presentation_of_clauses_spec cls prems concl :
     Clauses.In (prems, concl) cls ->
     In (NES.singleton concl ∨ prems, prems) (C (presentation_of_clauses cls)).
@@ -70,3 +97,170 @@
     intros ha c hin. specialize (ha c hin).
     now apply presentation_entails_valid.
   Qed.
+
+  Lemma completeness_eq_cstrs cstrs s t :
+    relations_of_constraints cstrs ⊢ℒ s ≡ t <->
+    entails_z_cstr cstrs (s, ConstraintType.Eq, t).
+  Proof.
+    unfold entails_z_cstr.
+    rewrite -entails_L_entails_ℋ_equiv.
+    rewrite -LoopCheck.Impl.Abstract.entails_L_rels_entails_L_clauses.
+    rewrite relation_of_constraint_of_clause //=.
+    now rewrite rels_of_z_constraints_spec entails_L_all_tip.
+  Qed.
+
+  Lemma completeness_le cstrs s t :
+    relations_of_constraints cstrs ⊢ℒ s ≤ t <->
+    entails_z_cstr cstrs (s, ConstraintType.Le, t).
+  Proof.
+    unfold entails_z_cstr.
+    split.
+    - move/completeness_eq_cstrs. cbn.
+      intros h; red in h. cbn in h.
+      eapply Theory.le_spec. now rewrite /Clauses.le.
+    - move/entails_ℋ_entails_L. apply entails_L_clauses_le.
+  Qed.
+
+
+
+  Lemma entails_clauses_le {cstrs l r} :
+    ZUnivConstraintSet.In (l, ConstraintType.Le, r) cstrs ->
+    of_z_constraints cstrs ⊢a r → l.
+  Proof.
+    intros hin l' cl.
+    eapply in_pred_closure_entails_clause, incls0.
+    rewrite of_z_constraints_spec. eexists; split; tea.
+    now apply in_clause_of_le.
+  Qed.
+
+  Lemma entails_clauses_eq_left {cstrs l r} :
+    ZUnivConstraintSet.In (l, ConstraintType.Eq, r) cstrs ->
+    of_z_constraints cstrs ⊢a r → l.
+  Proof.
+    intros hin l' cl.
+    eapply in_pred_closure_entails_clause, incls0.
+    rewrite of_z_constraints_spec. eexists; split; tea.
+    rewrite LoopCheck.to_clauses_spec. left. exists l'. split => //.
+  Qed.
+
+  Lemma entails_clauses_eq_right {cstrs l r} :
+    ZUnivConstraintSet.In (l, ConstraintType.Eq, r) cstrs ->
+    of_z_constraints cstrs ⊢a l → r.
+  Proof.
+    intros hin l' cl.
+    eapply in_pred_closure_entails_clause, incls0.
+    rewrite of_z_constraints_spec. eexists; split; tea.
+    rewrite LoopCheck.to_clauses_spec. right. exists l'. split => //.
+  Qed.
+
+  Lemma entails_clauses_eq_cstr {cstrs l r} :
+    ZUnivConstraintSet.In (l, ConstraintType.Eq, r) cstrs ->
+    of_z_constraints cstrs ⊢ℋ l ≡ r.
+  Proof.
+    intros hin.
+    apply Theory.eq_antisym.
+    split.
+    - rewrite to_entails_all. now apply entails_clauses_eq_left.
+    - rewrite to_entails_all. now apply entails_clauses_eq_right.
+  Qed.
+
+  Lemma entails_clauses_le_cstr {cstrs l r} :
+    ZUnivConstraintSet.In (l, ConstraintType.Le, r) cstrs ->
+    of_z_constraints cstrs ⊢ℋ l ⋞ r.
+  Proof.
+    intros hin.
+    rewrite to_entails_all. now apply entails_clauses_le.
+  Qed.
+
+  Lemma entails_L_clauses_eq_cstr {cstrs l r} :
+    ZUnivConstraintSet.In (l, ConstraintType.Eq, r) cstrs ->
+    relations_of_clauses (of_z_constraints cstrs) ⊢ℒ l ≡ r.
+  Proof.
+    move/entails_clauses_eq_cstr.
+    rewrite -entails_L_entails_ℋ_equiv.
+    now rewrite -(entails_L_clauses_entails_L_relations _ (l, r)).
+  Qed.
+
+  Lemma entails_L_clauses_le_cstr {cstrs l r} :
+    ZUnivConstraintSet.In (l, ConstraintType.Le, r) cstrs ->
+    relations_of_clauses (of_z_constraints cstrs) ⊢ℒ l ≤ r.
+  Proof.
+    move/entails_clauses_le_cstr.
+    rewrite -entails_L_entails_ℋ_equiv.
+    now rewrite /entails_L_clauses Clauses.entails_L_pres_clauses_of_le.
+  Qed.
+
+  Lemma entails_L_clauses_leq_def {p l r} :
+    entails_L_clauses p (l ⋞ r) <-> entails_L_clauses p (l ∨ r ≡ r).
+  Proof.
+    rewrite /entails_L_clauses.
+    rewrite entails_L_pres_clauses_of_relations_eq.
+    now rewrite Clauses.entails_L_pres_clauses_of_le.
+  Qed.
+
+    Lemma entails_to_clauses {prems concl cstr} :
+     Clauses.In (prems, concl) (LoopCheck.to_clauses cstr) ->
+     [relation_of_constraint cstr] ⊢ℒ (singleton concl ≤ prems).
+  Proof.
+    destruct cstr as [[l []] r].
+    - intros hin. cbn -[le].
+      have en := entails_L_relations_of_clauses_le l r.
+      setoid_rewrite <- en. cbn in hin.
+      now eapply entails_L_in_cls.
+    - intros hin; cbn in hin |- *.
+      rewrite -entails_L_relations_of_clauses_eq.
+      now eapply entails_L_in_cls.
+  Qed.
+
+  Lemma entails_L_clauses_all {cstrs s t} :
+    (relations_of_clauses (of_z_constraints cstrs)) ⊢ℒ s ≡ t <->
+    (relations_of_constraints cstrs) ⊢ℒ s ≡ t.
+  Proof.
+    now rewrite rels_of_z_constraints_spec.
+  Qed.
+
+  Lemma entails_L_clauses_le {cstrs s t} :
+    entails_L_pres_clauses (relations_of_clauses (of_z_constraints cstrs)) (s ⋞ t) ->
+    relations_of_constraints cstrs ⊢ℒ s ≤ t.
+  Proof.
+    intros hf. do 2 red in hf. rw_in clauses_of_le_spec hf.
+    eapply entails_L_split.
+    move=> le hin.
+    move: (hf (t, le)) => /fwd.
+    { exists le; split => //. }
+    move=> h; red in h. cbn in h.
+    now eapply entails_L_clauses_all in h.
+  Qed.
+
+  Lemma entails_L_clauses_of_eq {cstrs s t} :
+    entails_L_pres_clauses (relations_of_clauses (of_z_constraints cstrs)) (s ≡ t) ->
+    relations_of_constraints cstrs ⊢ℒ s ≡ t.
+  Proof.
+    intros hf. do 2 red in hf.
+    eapply entails_L_eq_antisym. split.
+    all: apply entails_L_clauses_le.
+    - intros cl hin; red. eapply hf.
+      rewrite /clauses_of_eq. clsets.
+    - intros cl hin; red. eapply hf.
+      rewrite /clauses_of_eq. clsets.
+  Qed.
+
+
+  Definition entails_L_cstr p c :=
+    let '(l, d, r) := c in
+    match d with
+    | ConstraintType.Le => p ⊢ℒ l ≤ r
+    | ConstraintType.Eq => p ⊢ℒ l ≡ r
+    end.
+
+  Lemma entails_L_clauses_cstr {cstrs c} :
+    entails_L_clauses (of_z_constraints cstrs) (LoopCheck.to_clauses c) ->
+    entails_L_cstr (relations_of_constraints cstrs) c.
+  Proof.
+    destruct c as [[l []] r].
+    - cbn. apply entails_L_clauses_le.
+    - cbn. apply entails_L_clauses_of_eq.
+  Qed.
+
+  Definition entails_L_cstrs p cstrs :=
+    ZUnivConstraintSet.For_all (entails_L_cstr p) cstrs.
